compilation.v : finis fixpoint traduction et correction du lemme de correction

compilation.v
@@ -1,41 +1,40 @@
 Load "CAM".
 Load "Lambda_Calcul".
 
+Notation "'appl'" := (app lambda_term).
+Notation "'consl'" := (cons lambda_term).
+Notation "'constantel'" := (constante lambda_term).
+Notation "'curl'" := (cur lambda_term).
+Notation "'fstl'" := (fst lambda_term).
+Notation "'pairel'" := (paire lambda_term).
+Notation "'pushl'" := (push lambda_term).
+Notation "'quotel'" := (quote lambda_term).
+Notation "'sndl'" := (snd lambda_term).
+Notation "'stackl'" := (stack lambda_term).
+Notation "'swapl'" := (swap lambda_term).
+
+Fixpoint acc (n : nat) : (code lambda_term) :=
+  match n with
+  | 0 => sndl :: nil
+  | S m => fstl :: (acc m)
+  end.
+
 Fixpoint traduction (t : lambda_term) : option (code lambda_term) :=
 match t with
-|variable n => Some ((quote lambda_term (variable n))::nil)
-|ref n => Some ((app lambda_term)::nil)  (*en attendant*)
-|abstraction u => match traduction u with
-    |Some C => Some ((cur lambda_term C)::nil)
+|variable n => Some ((quotel (variable n))::nil)
+|ref n => Some (acc n)
+|abstraction u =>
+    match traduction u with
+    | Some C => Some ((curl C)::nil)
     | _ => None
-    end
-|application u v => match u with
-    |abstraction x => match (traduction x, traduction v) with 
-        |(Some C, Some C1) => Some (((push lambda_term)::C1)++((cons lambda_term)::C))
-        | (_, _) => None
-        end
-    | _ => None
-    end
+  end
+|application u v =>
+    match (traduction u,traduction v) with
+    | (Some C, Some C1) => Some (pushl::(curl C)::swapl::nil ++ C1 ++ appl::nil)
+    | (_, _) => None
+  end
 end.
 
-Notation "'constantel'" := (constante lambda_term).
-Notation "'pairel'" := (paire lambda_term).
-Notation "'quotel'" := (quote lambda_term).
-Notation "'consl'" := (cons lambda_term).
-Notation "'appl'" := (app lambda_term).
 Definition empty_stack := (constantel (var 0))::nil.
 
-Goal forall c1 c2 : code lambda_term, traduction (lapp id (var 1)) = Some c1 -> traduction (var 1) = Some c2 -> cam_reduction_ref_trans lambda_term empty_stack c1 empty_stack c2.
-Proof.
-intros.
-inversion H; inversion H0.
-apply reduc_trans with
-((constantel (var 0))::(constantel (var 0))::nil)
-((quotel (var 1)) :: consl :: (appl) :: nil).
-apply reduc_cas_base; remove_simple_cam_reduc.
-apply reduc_trans with
-((constantel (var 1)) :: (constantel (var 0))::nil)
-(consl :: appl :: nil).
-apply reduc_cas_base; remove_simple_cam_reduc.
-
-Lemma correction : forall (t t' : lambda_term) (c1 c2 : code lambda_term), t ->β t' -> traduction t = Some c1 -> traduction t' = Some c2 -> cam_reduction_ref_trans lambda_term empty_stack c1 empty_stack c2.
+Lemma correction : forall (t t' : lambda_term) (c1 c2 : code lambda_term), t ->β t' -> traduction t = Some c1 -> traduction t' = Some c2 -> exists S : stackl, cam_reduction_ref_trans lambda_term empty_stack c1 S c2.
